verify.dfy
@@ -24,6 +24,8 @@ module verify {
     conn_ctx.Init();
     var tls_seq := new tls_opts_seq;
     tls_seq.Init();
+    // add tls_opts_client_setup - in connect cb
+    // connect_cb()
     var y := set_certificate_chain(tls_seq, conn_ctx, "filepath");
     //assert the crap out of it
     assert(y == 1);
@@ -33,14 +35,6 @@ module verify {
     // assert(|tls_opts_seq.opts_list| >= old(|tls_opts_seq.opts_list|))
 
     assert sock.Secure();
-
-    // TODO - when openssl is initialized for a socket, check that the following
-    // functions are called from OpenSSL
-    // SSL_library_init();
-    // OpenSSL_add_all_algorithms();
-    // ERR_load_BIO_strings();
-    // ERR_load_crypto_strings();
-    // SSL_load_error_strings();
   }
 
 }
